Instances/Setoid/CommMon.v
@@ -1,644 +1,185 @@
 From CoqAlgs.Sorting Require Import Perm InsertionSort.
 
 From Cat Require Export Cat.
-From Cat.Universal Require Import Initial Terminal Product Coproduct.
+From Cat.Universal Require Import Initial Terminal Zero Product Coproduct.
 From Cat Require Export Instances.Setoid.Mon.
 
 Set Implicit Arguments.
 
-Class ComMon : Type :=
+Class CMon : Type :=
 {
   mon :> Mon;
-  com : forall x y : mon, op x y == op y x
+  op_comm: forall x y : mon, op x y == op y x
 }.
 
 Arguments mon _ : clear implicits.
 
-Coercion mon : ComMon >-> Mon.
+Coercion mon : CMon >-> Mon.
 
-Inductive exp (X : ComMon) : Type :=
-| Id : exp X
-| Var : nat -> exp X
-| Op : exp X -> exp X -> exp X
-| Mor : forall A : ComMon, MonHom A X -> exp A -> exp X.
-
-Arguments Id {X}.
-Arguments Var {X} _.
-Arguments Op {X} _ _.
-Arguments Mor {X A} _ _.
-
-Fixpoint expDenote {X : ComMon} (env : nat -> X) (e : exp X) : X :=
-match e with
-| Id => neutr
-| Var n => env n
-| Op e1 e2 => op (expDenote env e1) (expDenote env e2)
-| Mor _ _ => neutr
-end.
-
-Fixpoint simplifyExp {X : ComMon} (e : exp X) : exp X :=
-match e with
-| Id => Id
-| Var v => Var v
-| Op e1 e2 =>
-  match simplifyExp e1, simplifyExp e2 with
-  | Id, e2' => e2'
-  | e1', Id => e1'
-  | e1', e2' => Op e1' e2'
-  end
-| Mor f e' =>
-  match simplifyExp e' with
-  | Id => Id
-  | Op e1 e2 => Op (Mor f e1) (Mor f e2)
-  | e'' => Mor f e''
-  end
-end.
-
-Lemma simplifyExp_correct :
-  forall (X : ComMon) (env : nat -> X) (e : exp X),
-    expDenote env (simplifyExp e) == expDenote env e.
-Proof.
-  induction e; cbn; [easy | easy | |].
-  - now destruct (simplifyExp e1), (simplifyExp e2); cbn in *;
-      rewrite <- ?IHe1, <- ?IHe2, ?neutr_l, ?neutr_r.
-  - now destruct (simplifyExp e); cbn in *; rewrite ?neutr_l.
-Qed.
-
-Fixpoint expDenoteL {X : ComMon} (env : nat -> X) (l : list nat) : X :=
-match l with
-| [] => neutr
-| h :: t => op (env h) (expDenoteL env t)
-end.
-
-Lemma expDenoteL_app :
-  forall (X : ComMon) (env : nat -> X) (l1 l2 : list nat),
-    expDenoteL env (l1 ++ l2) == op (expDenoteL env l1) (expDenoteL env l2).
-Proof.
-  induction l1 as [| h1 t1]; cbn; intros.
-  - now rewrite neutr_l.
-  - now rewrite <- assoc, IHt1.
-Qed.
-
-Fixpoint flatten {X : ComMon} (e : exp X) : list nat :=
-match e with
-| Id => []
-| Var v => [v]
-| Op e1 e2 => flatten e1 ++ flatten e2
-| Mor f e' => []
-end.
-
-Lemma flatten_correct :
-  forall (X : ComMon) (env : nat -> X) (e : exp X),
-    expDenoteL env (flatten e) == expDenote env e.
-Proof.
-  induction e; cbn; [easy | | |].
-  - now rewrite neutr_r.
-  - now rewrite expDenoteL_app, IHe1, IHe2.
-  - now rewrite ?expDenoteL_hom, ?IHe.
-Qed.
-
-Lemma expDenoteL_Permutation :
-  forall (X : ComMon) (env : nat -> X) (l1 l2 : list nat),
-    Permutation l1 l2 -> expDenoteL env l1 == expDenoteL env l2.
-Proof.
-  induction 1; cbn; [easy | | |].
-  - now rewrite IHPermutation.
-  - now rewrite !assoc, (com (env y)).
-  - now rewrite IHPermutation1, IHPermutation2.
-Qed.
-
-(* TOOD: fix *) Lemma sort_correct :
-  forall (X : ComMon) (env : nat -> X) (l : list nat) (s : Sort le),
-    expDenoteL env (s l) == expDenoteL env l.
-Proof.
-(*
-  intros. apply expDenoteL_Permutation. apply (perm_Permutation).
-  now rewrite <- sort_perm.
-Qed.
-*)
-Admitted.
-
-(* TODO: uncomment code on commutative monoid simplification *)
-(*
-Definition simplify {X : ComMon} (e : exp X) : list nat :=
-  insertionSort le (flatten (simplifyExp e)).
-
-Lemma simplify_correct :
-  forall (X : ComMon) (env : nat -> X) (e1 e2 : exp X),
-    expDenoteL env (simplify e1) == expDenoteL env (simplify e2) ->
-      expDenote env e1 == expDenote env e2.
-Proof.
-  unfold simplify. intros.
-  rewrite (@sort_correct X env (flatten (simplifyExp e1))
-                         (Sort_insertionSort natle)),
-          (@sort_correct X env (flatten (simplifyExp e2))
-                         (Sort_insertionSort natle))
-  in H.
-  now rewrite !flatten_correct, !simplifyExp_correct in H.
-Qed.
-
-Ltac inList x l :=
-match l with
-| [] => false
-| x :: _ => true
-| _ :: ?l' => inList x l'
-end.
-
-Ltac addToList x l :=
-  let b := inList x l in
-match b with
-| true => l
-| false => constr:(x :: l)
-end.
-
-Ltac lookup x l :=
-match l with
-| x :: _ => constr:(0)
-| _ :: ?l' => let n := lookup x l' in constr:(S n)
-end.
-
-Ltac allVars xs e :=
-match e with
-| op ?e1 ?e2 => let xs' := allVars xs e2 in allVars xs' e1
-| ?f ?e' => allVars xs e'
-| _ => addToList e xs
-end.
-
-Ltac reifyTerm env x :=
-match x with
-| neutr => constr:(Id)
-| op ?a ?b =>
-  let e1 := reifyTerm env a in
-  let e2 := reifyTerm env b in constr:(Op e1 e2)
-| _ => let n := lookup x env in constr:(Var n)
-end.
-
-Ltac functionalize l X :=
-let rec loop n l' :=
-  match l' with
-  | [] => constr:(fun _ : nat => @neutr X)
-  | ?h :: ?t =>
-    let f := loop (S n) t in
-    constr:(fun m : nat => if m =? n then h else f m)
-  end
-in loop 0 l.
-
-Ltac reify X :=
-match goal with
-| |- ?e1 == ?e2 =>
-  let xs := allVars constr:(@nil X) e1 in
-  let xs' := allVars xs e2 in
-  let r1 := reifyTerm xs' e1 in
-  let r2 := reifyTerm xs' e2 in
-  let env := functionalize xs' X in
-    change (expDenote env r1 == expDenote env r2)
-end.
-
-Ltac reifyEqv X env a b :=
-  let e1 := reifyTerm env a in
-  let e2 := reifyTerm env b in constr:((e1, e2)).
-
-(* TODO : improve reflection *)
-Lemma flat_reflect_goal :
-  forall (X : ComMon) (env : nat -> X) (e1 e2 : exp X),
-    flatten (simplifyExp e1) = flatten (simplifyExp e2) ->
-      expDenote env e1 == expDenote env e2.
-Proof.
-  intros.
-  apply simplify_correct; unfold simplify.
-  now rewrite H.
-Qed.
-
-Lemma flat_reflect_hyp :
-  forall (X : ComMon) (env : nat -> X) (e1 e2 : exp X),
-    expDenote env e1 == expDenote env e2 ->
-      flatten (simplifyExp e1) == flatten (simplifyExp e2).
-Proof.
-  now induction e1; destruct e2; cbn; intros.
-Qed.
-
-Lemma flat_reflect_hyp' :
-  forall (X : ComMon) (env : nat -> X) (e1 e2 : exp X) (s : Sort natle),
-    expDenote env e1 == expDenote env e2 ->
-      expDenoteL env (s (flatten (simplifyExp e1))) ==
-      expDenoteL env (s (flatten (simplifyExp e2))).
-Proof.
-  now intros; rewrite !sort_correct, !flatten_correct, !simplifyExp_correct.
-Qed.
-
-Ltac cmon_subst := repeat
-multimatch goal with
-| H : ?x == ?y |- _ => rewrite <- ?H in *
-| H : ?x == ?x |- _ => clear H
-end.
-
-Ltac reflect_cmon' := cbn; intros; cmon_subst;
-match goal with
-| X : ComMon |- ?e1 == ?e2 => reify X; apply simplify_correct; cbn; rewrite ?neutr_l, ?neutr_r
-end.
-
-Ltac reflect_cmon := reflect_cmon'; try reflexivity.
-
-Ltac reflect_goal := cbn; intros;
-match goal with
-| X : ComMon |- ?e1 == ?e2 => reify X; apply flat_reflect_goal
-end.
-
-(* Lemma cons_nil_all :
-  forall (A : Type) (h h' : A),
-    [h] = [h'] -> forall l : list A, cons h l = cons h' l.
-Proof.
-  now inversion 1.
-Qed. *)
-
-Goal forall (X : ComMon) (a b c : X),
-  op a (op b c) == op (op a b) c.
-Proof.
-  reflect_cmon.
-Qed.
-
-Goal forall (X : ComMon) (a b : X),
-  op a b == op b a.
-Proof.
-  reflect_cmon.
-Qed.
-
-Goal forall (X : ComMon) (a b b' c : X),
-  b == b' -> op a (op b c) == op (op a b') c.
-Proof.
-  now reflect_cmon'.
-Qed.
-
-Goal forall (X : ComMon) (a a' b b' c c' : X),
-  op a b == op a b' -> op (op a b) c == op b' (op a c).
-Proof.
-  reflect_cmon'. rewrite ?assoc. rewrite (com b').
-  rewrite !H. now reflect_cmon'.
-Qed.
-
-Goal forall (X : ComMon) (a a' b b' c c' : X),
-  a == b -> b == c -> c == a -> op b (op a c) == op a (op neutr (op b c)).
-Proof.
-  now reflect_cmon'.
-Qed.
-
-Inductive formula (X : ComMon) : Type :=
-| fVar   : Prop -> formula X
-| fEquiv : exp X -> exp X -> formula X
-| fNot   : formula X -> formula X
-| fAnd   : formula X -> formula X -> formula X
-| fOr    : formula X -> formula X -> formula X
-| fImpl  : formula X -> formula X -> formula X.
-
-Arguments fVar {X} _.
-
-Fixpoint formulaDenote {X : ComMon} (env : nat -> X) (p : formula X)
-  : Prop :=
-match p with
-| fVar P       => P
-| fEquiv e1 e2 => expDenote env e1 == expDenote env e2
-| fNot p'      => ~ formulaDenote env p'
-| fAnd p1 p2   => formulaDenote env p1 /\ formulaDenote env p2
-| fOr p1 p2    => formulaDenote env p1 \/ formulaDenote env p2
-| fImpl p1 p2  => formulaDenote env p1 -> formulaDenote env p2
-end.
-
-Ltac allVarsFormula xs P :=
-match P with
-| ?a == ?b => allVars xs P
-| ~ ?P' => allVarsFormula xs P'
-| ?P1 /\ ?P2 => let xs' := allVarsFormula xs P1 in allVarsFormula xs' P2
-| ?P1 \/ ?P2 => let xs' := allVarsFormula xs P1 in allVarsFormula xs' P2
-| ?P1 -> ?P2 => let xs' := allVarsFormula xs P1 in allVarsFormula xs' P2
-| _ => xs
-end.
-
-Ltac reifyFormula X xs P :=
-match P with
-| ~ ?P' => let e := reifyFormula X xs P' in constr:(fNot e)
-| ?a == ?b =>
-  let e1 := reifyTerm xs a in
-  let e2 := reifyTerm xs b in constr:(fEquiv e1 e2)
-| ?P1 /\ ?P2 =>
-  let e1 := reifyFormula X xs P1 in
-  let e2 := reifyFormula X xs P2 in constr:(fAnd e1 e2)
-| ?P1 \/ ?P2 =>
-  let e1 := reifyFormula X xs P1 in
-  let e2 := reifyFormula X xs P2 in constr:(fOr e1 e2)
-| ?P1 -> ?P2 =>
-  let e1 := reifyFormula X xs P1 in
-  let e2 := reifyFormula X xs P2 in constr:(fImpl e1 e2)
-| _ => constr:(fVar X P)
-end.
-
-Ltac reifyGoal :=
-match goal with
-| X : ComMon |- ?P =>
-  let xs := allVarsFormula constr:(@nil X) P in
-  let env := functionalize xs X in
-  let e := reifyFormula X xs P in change (formulaDenote env e)
-end.
-
-Definition list_eq :
-  forall (l1 l2 : list nat), {l1 = l2} + {l1 <> l2}.
-Proof.
-  do 2 decide equality.
-Defined.
-
-Fixpoint solveFormula {X : ComMon} (env : nat -> X) (f : formula X)
-  : option (formulaDenote env f).
-Proof.
-  destruct f; cbn.
-  - apply None.
-  - destruct (list_eq
-              (insertionSort natle (flatten (simplifyExp e)))
-              (insertionSort natle (flatten (simplifyExp e0)))).
-    + apply Some. now apply simplify_correct.
-    + apply None.
-  - apply None.
-  - destruct (solveFormula X env f1), (solveFormula X env f2).
-    + now apply Some.
-    + apply None.
-    + apply None.
-    + apply None.
-  - destruct (solveFormula X env f1).
-    + apply Some. now left.
-    + destruct (solveFormula X env f2).
-      * apply Some. now right.
-      * apply None.
-  - destruct (solveFormula X env f2).
-    + apply Some. now intro.
-    + apply None.
-Defined.
-
-Lemma solveFormula_spec :
-  forall (X : ComMon) (env : nat -> X) (f : formula X),
-    (exists p : formulaDenote env f, solveFormula env f = Some p) ->
-      formulaDenote env f.
-Proof.
-  now intros; destruct H.
-Qed.
-
-Ltac solve_goal' :=
-  cbn; intros; cmon_subst; reifyGoal;
-  apply solveFormula_spec; cbn; eauto.
-
-Ltac solve_goal :=
-  try (solve_goal'; fail);
-  fail "Cannot solve the goal".
-
-Goal forall (X : ComMon) (a a' b b' c c' : X),
-  a == b -> b == c -> c == a -> a == c /\ op c c == op b b.
-Proof.
-  solve_goal.
-Qed.
-
-Goal forall (X : ComMon) (a a' b b' c c' : X),
-  a == b -> b' == c' -> 2 = 2 \/ op c c == op c (op a c').
-Proof.
-  intros X a _ b b' c c'.
-  now match goal with
-  | X : ComMon |- ?P =>
-    let xs := allVarsFormula constr:(@nil X) P in
-    let env := functionalize xs X in
-    let f := fresh "f" in
-    let f' := constr:(@formulaDenote X env) in pose f' as f
-  end; cbn in *.
-Abort.
-*)
-
-(*
-#[refine]
 #[export]
-Instance MonHomSetoid (X Y : Mon) : Setoid (MonHom X Y) :=
+Instance CMonCat : Cat :=
 {
-  equiv := fun f g : MonHom X Y =>
-    @equiv _ (SgrHomSetoid X Y) f g
-}.
-Proof. now apply Setoid_kernel_equiv. Defined.
-
-Definition MonComp (X Y Z : Mon) (f : MonHom X Y) (g : MonHom Y Z)
-    : MonHom X Z.
-Proof.
-  now exists (SgrComp f g).
-Defined.
-
-Definition MonId (X : Mon) : MonHom X X.
-Proof.
-  now exists (SgrId X).
-Defined.
-
-#[refine]
-#[export]
-Instance MonCat : Cat :=
-{
-  Ob := Mon;
+  Ob := CMon;
   Hom := MonHom;
   HomSetoid := MonHomSetoid;
   comp := MonComp;
-  id := MonId
+  id := MonId;
+  Proper_comp := @Proper_comp MonCat;
+  comp_id_l := @comp_id_l MonCat;
+  comp_id_r := @comp_id_r MonCat;
+  comp_assoc := @comp_assoc MonCat;
 }.
-Proof. all: now mon. Defined.
 
 #[refine]
 #[export]
-Instance Mon_init : Mon :=
+Instance CMon_init : CMon :=
 {
-  sgr := Sgr_term;
-  neutr := tt
+  mon := Mon_init;
 }.
-Proof. all: now mon. Defined.
+Proof. easy. Defined.
 
-Definition Mon_Setoid_create (X : Mon) : SetoidHom Mon_init X.
-Proof.
-  now exists (fun _ => neutr).
-Defined.
-
-Definition Mon_Sgr_create (X : Mon) : SgrHom Mon_init X.
-Proof.
-  now exists (Mon_Setoid_create X).
-Defined.
-
-Definition Mon_create (X : Mon) : Hom Mon_init X.
-Proof.
-  now exists (Mon_Sgr_create X).
-Defined.
+#[export]
+Instance HasInit_CMon : HasInit CMonCat :=
+{
+  init := CMon_init;
+  create := Mon_create;
+  isInitial_HasInit' := @isInitial_HasInit' MonCat _;
+}.
 
 #[refine]
 #[export]
-Instance HasInit_Mon : HasInit MonCat :=
+Instance CMon_term : CMon :=
 {
-  init := Mon_init;
-  create := Mon_create
+  mon := Mon_term;
 }.
-Proof. now mon. Defined.
+Proof. easy. Defined.
+
+#[export]
+Instance HasTerm_CMon : HasTerm CMonCat :=
+{
+  term := CMon_term;
+  delete := Mon_delete;
+  isTerminal_HasTerm' := @isTerminal_HasTerm' MonCat _;
+}.
 
 #[refine]
 #[export]
-Instance Mon_term : Mon :=
+Instance HasZero_CMon : HasZero CMonCat :=
 {
-  sgr := Sgr_term;
-  neutr := tt
+  HasInit_HasZero := HasInit_CMon;
+  HasTerm_HasZero := HasTerm_CMon
 }.
-Proof. all: now mon. Defined.
-
-Definition Mon_Setoid_delete (X : Mon) : SetoidHom X Mon_term.
-Proof.
-  now exists (fun _ => tt).
-Defined.
-
-Definition Mon_Sgr_delete (X : Mon) : SgrHom X Mon_term.
-Proof.
-  now exists (Mon_Setoid_delete X).
-Defined.
-
-Definition Mon_delete (X : Mon) : Hom X Mon_term.
-Proof.
-  now exists (Mon_Sgr_delete X).
-Defined.
+Proof. easy. Defined.
 
 #[refine]
 #[export]
-Instance HasTerm_Mon : HasTerm MonCat :=
+Instance CMon_product (A B : CMon) : CMon :=
 {
-  term := Mon_term;
-  delete := Mon_delete
+  mon := Mon_product A B;
 }.
-Proof. now mon. Defined.
-
-#[refine]
-#[export]
-Instance HasZero_Mon : HasZero MonCat :=
-{
-    HasInit_HasZero := HasInit_Mon;
-    HasTerm_HasZero := HasTerm_Mon
-}.
-Proof. now mon. Defined.
-
-#[refine]
-#[export]
-Instance Mon_product (X Y : Mon) : Mon :=
-{
-  sgr := Sgr_product X Y;
-  neutr := (neutr, neutr);
-}.
-Proof. all: now destruct a; mon. Defined.
-
-Definition Mon_outl (X Y : Mon) : Hom (Mon_product X Y) X.
 Proof.
-  now exists (Sgr_outl X Y).
-Defined.
-
-Definition Mon_outr (X Y : Mon) : Hom (Mon_product X Y) Y.
-Proof.
-  now exists (Sgr_outr X Y).
-Defined.
-
-Definition Mon_fpair (A B X : Mon) (f : MonHom X A) (g : MonHom X B)
-    : MonHom X (Mon_product A B).
-Proof.
-  now exists (Sgr_fpair f g).
+  intros [a1 b1] [a2 b2]; cbn.
+  now split; apply op_comm.
 Defined.
 
 #[refine]
 #[export]
-Instance HasProducts_Mon : HasProducts MonCat :=
+Instance HasProducts_CMon : HasProducts CMonCat :=
 {
-  product := Mon_product;
+  product := CMon_product;
   outl := Mon_outl;
   outr := Mon_outr;
-  fpair := Mon_fpair
+  fpair := Mon_fpair;
 }.
 Proof.
-  now repeat split; cat.
+  now repeat split; cbn in *.
+Defined.
+
+#[export]
+Instance CMon_coproduct (A B : CMon) : CMon := CMon_product A B.
+
+Definition CMon_finl' (A B : CMon) : SetoidHom A (CMon_coproduct A B).
+Proof.
+  esplit. Unshelve. all: cycle 1.
+  - exact (fun a => (a, neutr)).
+  - now intros x y Heq; cbn.
+Defined.
+
+Definition CMon_finl (A B : CMon) : MonHom A (CMon_coproduct A B).
+Proof.
+  esplit. Unshelve. all: cycle 1.
+  - esplit with (CMon_finl' A B); cbn.
+    now intros; rewrite neutr_l.
+  - easy.
+Defined.
+
+Definition CMon_finr' (A B : CMon) : SetoidHom B (CMon_coproduct A B).
+Proof.
+  esplit. Unshelve. all: cycle 1.
+  - exact (fun b => (neutr, b)).
+  - now intros x y Heq; cbn.
+Defined.
+
+Definition CMon_finr (A B : CMon) : MonHom B (CMon_coproduct A B).
+Proof.
+  esplit. Unshelve. all: cycle 1.
+  - esplit with (CMon_finr' A B); cbn.
+    now intros; rewrite neutr_l.
+  - easy.
+Defined.
+
+#[export]
+Instance CMon_copair'
+  {A B X : CMon} (f : MonHom A X) (g : MonHom B X) : SetoidHom (CMon_coproduct A B) X.
+Proof.
+  esplit. Unshelve. all: cycle 1.
+  - refine (fun '(a, b) => op (f a) (g b)).
+  - now intros [a1 b1] [a2 b2]; cbn; intros [-> ->].
+Defined.
+
+#[export]
+Instance CMon_copair
+  {A B X : CMon} (f : MonHom A X) (g : MonHom B X) : MonHom (CMon_coproduct A B) X.
+Proof.
+  esplit. Unshelve. all: cycle 1.
+  - esplit with (CMon_copair' f g); cbn.
+    intros [a1 b1] [a2 b2]; cbn.
+    rewrite !pres_op.
+    rewrite !assoc; f_equiv.
+    rewrite <- !assoc; f_equiv.
+    apply op_comm.
+  - now cbn; rewrite !pres_neutr, neutr_l.
 Defined.
 
 #[refine]
 #[export]
-Instance forgetful : Functor MonCat CoqSetoid :=
+Instance HasCoproducts_CMon : HasCoproducts CMonCat :=
 {
-  fob := fun X : Mon => @setoid (sgr X);
+  coproduct := CMon_coproduct;
+  finl := CMon_finl;
+  finr := CMon_finr;
+  copair := @CMon_copair;
 }.
 Proof.
-  - now cbn; intros; exact X.
-  - formulaer. all: mon.
+  split; cbn.
+  - now intros; rewrite pres_neutr, neutr_r.
+  - now intros; rewrite pres_neutr, neutr_l.
+  - intros P' h1 h2 HA HB [a b]; cbn.
+    assert (Heq :
+        h1 (@op (CMon_coproduct A B) (a, neutr) (neutr, b))
+          ==
+        h2 (@op (CMon_coproduct A B) (a, neutr) (neutr, b)))
+      by now rewrite !pres_op; f_equiv.
+    now cbn in Heq; rewrite neutr_l, neutr_r in Heq.
 Defined.
-
-Notation "'U'" := forgetful.
-
-Definition free_monoid
-  (X : Ob CoqSetoid) (M : Mon) (p : Hom X (fob U M)) : Prop :=
-    forall (N : Mon) (q : SetoidHom X (fob U N)),
-      exists!! h : MonHom M N, q == p .> fmap U h.
 
 #[refine]
 #[export]
-Instance MonListUnit_Setoid' : Setoid' :=
+Instance forgetful : Functor CMonCat MonCat :=
 {
-  carrier := nat;
-  setoid := {| equiv := eq |}
-}.
-
-#[refine]
-#[export]
-Instance MonListUnit : Mon :=
-{
-  sgr :=
-  {|
-    setoid := MonListUnit_Setoid';
-    op := plus
-  |};
-  neutr := 0
+  fob := mon;
 }.
 Proof.
-  all: now cbn; intros; ring.
+  - easy.
+  - easy.
 Defined.
-
-Definition MonListUnit_p : SetoidHom CoqSetoid_term MonListUnit.
-Proof.
-  now exists (fun _ => 1); formulaer.
-Defined.
-
-Lemma free_monoid_MonListUnit :
-  @free_monoid CoqSetoid_term MonListUnit MonListUnit_p.
-Proof.
-  unfold free_monoid. intros.
-  (*pose f1 : SetoidHom MonListUnit N :=
-  {|
-    func := fix f n : N :=
-    match n with
-    | 0 => @neutr N
-    | S n' => op (q tt) (f n')
-    end;
-    Proper_func := ltac: (formulaer; subst; easy)
-  |}.
-  pose f2 : SgrHom MonListUnit N :=
-  {|
-    setoidHom := @f1;
-    pres_op := ltac:(mon)
-  |}.*)
-  Definition f1 (N : Mon) (q : SetoidHom CoqSetoid_term (fob U N))
-    : SetoidHom MonListUnit N.
-    exists (fix f (n : nat) : N :=
-      match n with
-      | 0 => @neutr N
-      | S n' => op (q tt) (f n')
-      end).
-    formulaer. now subst.
-  Defined.
-  Definition f2 (N : Mon) (q : SetoidHom CoqSetoid_term (fob U N))
-    : SgrHom MonListUnit N.
-    exists (f1 N q). induction x as [| x']. simpl.
-      mon.
-      simpl. intro. now rewrite <- assoc, -> IHx'.
-  Defined.
-  Definition f3 (N : Mon) (q : SetoidHom CoqSetoid_term (fob U N))
-    : MonHom MonListUnit N.
-    exists (f2 N q). mon.
-  Defined.
-  exists (f3 N q). repeat split.
-    simpl. destruct x. mon.
-    destruct y, sgrHom0; cbn in *; intros ? n. induction n as [| n'].
-      mon.
-      pose (H' := pres_op). specialize (H' n' 1). rewrite plus_comm in H'.
-        rewrite H'. rewrite -> pres_op in H'. rewrite <- H', IHn'. f_equiv; mon.
-Defined.*)
